\documentclass[class=jsarticle, crop=false, dvipdfmx, fleqn]{standalone}
\input{../../../preamble}
\begin{document}
\section{}

\begin{align}
    & \bm{x}_i \in \mathbb{R}^{d},\ \bm{T} \in \mathbb{R}^{m \times d},\ \bm{W} \in \mathbb{R}^{n \times n},\ \bm{W}^\mathrm{T} = \bm{W} \\
    & \bm{X} = \qty(\bm{x}_1,\ \cdots,\ \bm{x}_n) \\
    & \bm{D} = \mathrm{diag}\qty(\sum_{i' = 1}^{n} W_{i, i'}) \\
    & \bm{L} = \bm{D} - \bm{W}
\end{align}
に対し，
\begin{equation}
    \sum_{i, i' = 1}^{n} W_{i, i'} ||\bm{T} \bm{x}_i - \bm{T} \bm{x}_{i'}||^2 = 2 \mathrm{tr}\qty(\bm{TXL}\bm{X}^\mathrm{T} \bm{T}^\mathrm{T})
    \label{eq:objective}
\end{equation}
が成立することを示す。

いま，
\begin{equation}
    \bm{z}_i = \bm{T} \bm{x}_i
\end{equation}
とおくと，
\begin{align*}
    \sum_{i, i' = 1}^{n} W_{i, i'} ||\bm{T} \bm{x}_i - \bm{T} \bm{x}_{i'}||^2
        & = \sum_{i, i' = 1}^{n} W_{i, i'} ||\bm{z}_i - \bm{z}_{i'}||^2 \\
        & = \sum_{i, i' = 1}^{n} W_{i, i'} (\bm{z}_i - \bm{z}_{i'})^\mathrm{T} (\bm{z}_i - \bm{z}_{i'}) \\
        & = \sum_{i, i' = 1}^{n} W_{i, i'} \qty{||\bm{z}_i||^2 + ||\bm{z}_{i'}||^2 - 2 \bm{z}_i^\mathrm{T} \bm{z}_{i'}}
\end{align*}
ここで，\(W_{i, i'} = W_{i', i}\)なので，
\begin{align}
    \sum_{i, i' = 1}^{n} W_{i, i'} ||\bm{T} \bm{x}_i - \bm{T} \bm{x}_{i'}||^2
        & = 2 \sum_{i, i' = 1}^{n} W_{i, i'} \qty(||\bm{z}_i||^2 - \bm{z}_i^\mathrm{T} \bm{z}_{i'}) \notag \\
        & = 2 \qty{\sum_{i=1}^{n} \qty(\sum_{i'=1}^{n} W_{i,i'} ||\bm{z}_i||^2) - \sum_{i, i' = 1}^{n} W_{i, i'} \bm{z}_i^\mathrm{T} \bm{z}_{i'}}
        \label{eq:inter}
\end{align}
いま，
\begin{equation}
    \bm{Z} = \qty(\bm{z}_1,\ \cdots,\ \bm{z}_n)
\end{equation}
を考えると，
\begin{equation}
    \mathrm{tr}\qty(\bm{ZDZ}^\mathrm{T}) = \sum_{i=1}^{n} \qty(\sum_{i'=1}^{n} W_{i,i'} ||\bm{z}_i||^2)
    \label{eq:ZDZ}
\end{equation}
となり，
また，
\begin{equation}
    \mathrm{tr}\qty(\bm{ZWZ}^\mathrm{T}) = \sum_{i, i' = 1}^{n} W_{i, i'} \bm{z}_i^\mathrm{T} \bm{z}_{i'}
    \label{eq:ZWZ}
\end{equation}
となる。

式(\ref{eq:inter})，(\ref{eq:ZDZ})，(\ref{eq:ZWZ})と\(\bm{Z} = \bm{TX}\)より，
\begin{align}
    \sum_{i, i' = 1}^{n} W_{i, i'} ||\bm{T} \bm{x}_i - \bm{T} \bm{x}_{i'}||^2
        & = 2\mathrm{tr}\qty(\bm{ZDZ}^\mathrm{T}) - 2\mathrm{tr}\qty(\bm{ZWZ}^\mathrm{T}) \\
        & = 2\mathrm{tr}\qty(\bm{ZLZ}^\mathrm{T}) \\
        & = 2 \mathrm{tr}\qty(\bm{TXL}\bm{X}^\mathrm{T} \bm{T}^\mathrm{T})
\end{align}
となって，式(\ref{eq:objective})が示された。





\end{document}
