\documentclass[class=jsarticle, crop=false, dvipdfmx, fleqn]{standalone}
\input{../../../preamble}
\begin{document}
\section{}

\(B_{\tau} (y)\)を再帰的に表現する。
\begin{align}
    B_{\tau} (y)
        & =
            \sum_{ y^{(\tau + 1)}, \ldots , y^\mathrm{(m)} = 1 }^{c}
            \exp(
                \sum_{k=\tau + 2}^{m} \bm{\zeta}^\mathrm{T} \bm{\varphi}_i^{(k)} \qty(y^{(k)},\ y^{(k-1)})
                + \bm{\zeta}^\mathrm{T} \bm{\varphi}_i^{(\tau + 1)} \qty(y^{(\tau + 1)},\ y)
                ) \\
        & =
            \sum_{y^(\tau + 1) = 1}^{c} \cdot \sum_{ y^{(\tau + 2)}, \ldots , y^\mathrm{(m)} = 1 }^{c}
            \exp{\sum_{k=\tau + 2}^{m} \bm{\zeta}^\mathrm{T} \bm{\varphi}_i^{(k)} \qty(y^{(k)},\ y^{(k-1)})}
            \exp(\bm{\zeta}^\mathrm{T} \bm{\varphi}_i^{(\tau + 1)} \qty(y^{(\tau + 1)},\ y))
\end{align}
ここで，
\begin{align}
    & \sum_{ y^{(\tau + 2)}, \ldots , y^\mathrm{(m)} = 1 }^{c}
        \exp{\sum_{k=\tau + 2}^{m} \bm{\zeta}^\mathrm{T} \bm{\varphi}_i^{(k)} \qty(y^{(k)},\ y^{(k-1)})} \notag \\
    & \ \qquad =
        \sum_{ y^{(\tau + 2)}, \ldots , y^\mathrm{(m)} = 1 }^{c}
            \exp{
                \sum_{k=\tau + 3}^{m} \bm{\zeta}^\mathrm{T} \bm{\varphi}_i^{(k)} \qty(y^{(k)},\ y^{(k-1)})
                + \bm{\zeta}^\mathrm{T} \bm{\varphi}_i^{(\tau + 2)} \qty(y^{(\tau + 2)},\ y^{(\tau + 1)})
                } \\
    & \ \qquad =
        B_{\tau + 1}\qty(y^{(\tau + 1)})
\end{align}
となるから，結局\(B_{\tau} (y)\)は，
\begin{equation}
    B_{\tau} (y) = \sum_{y^(\tau + 1) = 1}^{c} B_{\tau + 1}\qty(y^{(\tau + 1)}) \exp(\bm{\zeta}^\mathrm{T} \bm{\varphi}_i^{(\tau + 1)} \qty(y^{(\tau + 1)},\ y))
\end{equation}
という形で再帰表現される。


\end{document}
